Almost done with algorithms_modified proof of linear_search

theories/algos/algorithms.pas
@@ -1,0 +1,132 @@
+{$INLINE OFF}
+program Algorithms;
+
+uses
+    sysutils;
+
+type
+    int_arr = array of integer;
+
+var
+    arr, sorted: int_arr;
+    i: cardinal;
+    key: integer;
+
+procedure print_arr(arr : int_arr);
+var
+    i: cardinal;
+begin
+    write('[');
+    for i := 0 to high(arr) do
+    begin
+        write(inttostr(arr[i]));
+        if i <> high(arr) then
+            write(', ');
+    end;
+    writeln(']');
+end;
+
+function bubble_sort(arr: int_arr) : int_arr;
+var
+    temp: integer;
+    i, j: cardinal;
+begin
+    // Setup array
+    setlength(bubble_sort, length(arr));
+    for i := 0 to high(arr) do
+    begin
+        bubble_sort[i] := arr[i];
+    end;
+    
+    // Do sort
+    for i := high(bubble_sort) - 1 downto 0 do
+    begin
+        for j := 0 to i do 
+        begin
+            if bubble_sort[j] > bubble_sort[j + 1] then
+            begin
+                temp := bubble_sort[j];
+                bubble_sort[j] := bubble_sort[j + 1];
+                bubble_sort[j + 1] := temp;
+            end;
+        end;
+    end;
+
+    bubble_sort := bubble_sort;
+end;
+
+procedure simple_loop;
+var
+    i: cardinal;
+begin
+    for i := 0 to 10 do
+        writeln(i);
+end;
+
+function linear_search(arr: int_arr; key: integer) : integer;
+var
+    i: integer;
+begin
+    linear_search := -1;
+
+    for i := 0 to high(arr) do 
+    begin
+        if (arr[i] = key) then 
+        begin
+            linear_search := i;
+            break;
+        end;
+    end;
+end;
+
+function binary_search(arr: int_arr; key: integer) : integer;
+var
+    l, r, m: cardinal;
+begin
+    l := 0;
+    r := high(arr);
+
+    binary_search := -1;
+
+    while l <= r do
+    begin
+        m := l + (r - l) div 2;
+        if (arr[m] = key) then 
+        begin
+            binary_search := m;
+            break;
+        end;
+
+        if (arr[m] < key) then 
+            l := m + 1
+        else
+            r := m - 1;
+    end;
+end;
+
+begin
+    // Initialize array with random elements
+    setlength(arr, 100);
+    for i := 0 to high(arr) do
+        arr[i] := random(1000);
+
+    // Get key to search for, should be random
+    key := arr[50];
+
+    // Sort array to lost index of 50
+    sorted := bubble_sort(arr);
+
+    // Linear search
+    i := linear_search(sorted, key);
+    writeln('Linear search:');
+    writeln('  Key:        ', key);
+    writeln('  Index:      ', i);
+    writeln('  arr[index]: ', sorted[i]);
+
+    // Binary search
+    i := binary_search(sorted, key);
+    writeln('Binary search:');
+    writeln('  Key:        ', key);
+    writeln('  Index:      ', i);
+    writeln('  arr[index]: ', sorted[i]);
+end.
