vp_lifter/lib/generator_values.ml
@@ -1,0 +1,503 @@
+open Converter
+open String_utils
+open Parse_tree
+open Logging
+
+let preamble extract extract_lang =
+  let coq_extraction_dep s =
+    "Extr" ^ String.capitalize_ascii (String.lowercase_ascii extract_lang) ^ s
+  in
+  let ex =
+    if extract then "Extraction Language " ^ extract_lang ^ "." else ""
+  in
+  let req_imps =
+    List.map
+      (fun x -> "Require Import " ^ x ^ ".")
+      ( ["Volpic_preamble"; "String"; "ZArith"; "List"; "Bool"]
+      @
+      if extract then [coq_extraction_dep "Basic"; coq_extraction_dep "String"]
+      else [] )
+  in
+  let scopes =
+    List.map
+      (fun x -> "Open Scope " ^ x ^ ".")
+      ["string_scope"; "Z_scope"; "vp_scope"]
+  in
+  let imports = List.map (fun x -> "Import " ^ x ^ ".") ["ListNotations"] in
+  econcat "\n"
+    (comment "Preamble" :: List.concat [req_imps; [ex]; scopes; imports])
+  ^ "\n\n"
+
+let lang_ext l =
+  match String.lowercase_ascii l with
+  | "ocaml" ->
+      "ml"
+  | "haskell" ->
+      "hs"
+  | _ ->
+      failwith "Unexpected language " ^ l
+
+let sanitize_id id =
+  let replacements = [("$", "")] in
+  let id =
+    List.fold_left
+      (fun acc (rexp, repl) ->
+        Str.global_replace (Str.regexp_string rexp) repl acc )
+      id replacements
+  in
+  if contains id ":" then string_before_substr id ":" else id
+
+let extraction fn func lang path =
+  let path =
+    if path = "" then
+      econcat ""
+        [Filename.basename (Filename.remove_extension fn); "."; lang_ext lang]
+    else path
+  in
+  econcat " " ["Extraction"; "\"" ^ path ^ "\""; func ^ "."]
+
+let typctx = ref fresh_gamma
+
+(* This returns a string containing the Coq type representation of a variable *)
+let type_of_expr = function
+  | Identifier id ->
+      _log Log_Debug
+        ("Getting type of " ^ id ^ ": " ^ string_of_coq_type (!typctx id)) ;
+      !typctx id
+  | Integer _ | Add _ | Sub _ ->
+      Z
+  | Gt _ | Lt _ | Eq _ ->
+      Bool
+  | String _ ->
+      String
+  | ProcCall _ ->
+      Unit
+  | FuncCall (_, typ, _) ->
+      coq_type_of_return_type_root typ
+  | Subscript (rtr, _, _) ->
+      coq_type_of_return_type_root (rtr_of_rt rtr)
+  | Nothing ->
+      Unit
+
+let lcontains l i = List.exists (fun x -> x = i) l
+
+let default_coq_value = function
+  | Z ->
+      parens (econcat " " [int_expr_constr; "0"])
+  | _ ->
+      "VNull"
+
+let constr_of_coq_type = function
+  | Z ->
+      int_expr_constr
+  | String ->
+      str_expr_constr
+  | Unit ->
+      failwith "Shouldn't be trying to store a unit"
+  | Record ->
+      failwith "Can't store records yet"
+  | Bool ->
+      bool_expr_constr
+  | Vector _ ->
+      failwith "Can't store vectors yet"
+  | Error ->
+      failwith "Shouldn't be trying to store an error"
+
+let rec string_of_expr x shallow bound_vars =
+  let binop op e1 e2 =
+    string_of_expr e1 shallow bound_vars
+    ^ " " ^ op ^ " "
+    ^ string_of_expr e2 shallow bound_vars
+  in
+  match x with
+  | Identifier id ->
+      (* if lcontains bound_vars id then id
+         else *)
+      econcat " "
+        [ (* (if shallow then "" else coq_expr_type_getter (Identifier id))
+             ; *)
+          sf_get
+        ; store_name
+        ; "\"" ^ id_prefix ^ id ^ "\"" ]
+  | Subscript (rt, arr, idx) ->
+      econcat " "
+        [ "subscript"
+        ; parens (string_of_expr arr shallow bound_vars)
+        ; parens (string_of_expr idx shallow bound_vars)
+        ; default_coq_value (coq_type_of_return_type_root (rtr_of_rt rt)) ]
+  | Integer n ->
+      constr_of_coq_type Z ^ " " ^ string_of_int n
+  | String s ->
+      constr_of_coq_type String ^ " \"" ^ s ^ "\""
+  | Add (e1, e2) ->
+      binop "+" e1 e2
+  | Sub (e1, e2) ->
+      binop "-" e1 e2
+  | Gt (e1, e2) ->
+      binop ">?" e1 e2
+  | Lt (e1, e2) ->
+      binop "<?" e1 e2
+  | Eq (e1, e2) ->
+      binop "=?" e1 e2
+  | ProcCall (id, e) ->
+      econcat " "
+        ( sanitize_id id :: store_name
+        :: List.map
+             (fun s ->
+               let se = string_of_expr s shallow bound_vars in
+               if contains se " " then parens se else se )
+             e )
+  | FuncCall (func_name, rt, e) ->
+      econcat " "
+        [ (* coq_type_getter (coq_type_of_return_type_root rt)
+             ; *)
+          ( (* (match rt with Record _ -> "" | _ -> sf_get ^ " ")
+                 ^ *)
+            parens
+              (econcat " "
+                 ( sanitize_id func_name :: store_name
+                 :: List.map
+                      (fun s ->
+                        let se = string_of_expr s shallow bound_vars in
+                        if contains se " " then parens se else se )
+                      e ) )
+          ^ match rt with Record _ -> "" | _ -> " " ^ stringify "result" )
+        ; (match rt with Record _ -> stringify "result" | _ -> "") ]
+  | Nothing ->
+      ""
+
+and coq_type_getter = function
+  | Z ->
+      "get_int"
+  | Bool ->
+      "get_bool"
+  | String ->
+      "get_string"
+  | Vector s ->
+      "get_array"
+  | Record ->
+      ""
+  | Unit ->
+      failwith "Shouldn't be calling a getter for unit-type expr"
+  | Error ->
+      failwith "Couldn't retrieve type"
+
+and coq_expr_type_getter e = coq_type_getter (type_of_expr e)
+
+let store_string_of_return_type rtr =
+  match rtr with
+  | Dword ->
+      int_expr_constr
+  | Record s ->
+      comment ("record" ^ s)
+  | _ ->
+      failwith
+        ( "RTR "
+        ^ string_of_return_type_root rtr
+        ^ " not yet supported in store_string_of_expr" )
+
+let store_constr expr =
+  match expr with
+  | Identifier id ->
+      constr_of_coq_type (!typctx id)
+  | Integer _ | Add _ | Sub _ ->
+      int_expr_constr
+  | Gt _ | Lt _ | Eq _ ->
+      bool_expr_constr
+  | String _ ->
+      str_expr_constr
+  | ProcCall _ ->
+      unit_expr_constr
+  | FuncCall (_, rt, _) ->
+      store_string_of_return_type rt
+  | Subscript (rt, _, _) ->
+      store_string_of_return_type (rtr_of_rt rt)
+  | Nothing ->
+      failwith "Shouldn't be trying to store a Nothing"
+
+let store_string_of_expr e bound_vars =
+  parens (string_of_expr e false bound_vars)
+(* "("
+   ^ econcat " " [store_constr e; "("; string_of_expr e false bound_vars; ")"]
+   ^ ")" *)
+
+let rec loop condition body post depth =
+  econcat " "
+    [ parens
+        (econcat " "
+           [ "fix"
+           ; "loop"
+           ; parens (vp_depth ^ " : nat")
+           ; parens (broken ^ " : bool")
+           ; parens (store_name ^ " : store")
+           ; ":="
+           ; "\n"
+           ; matchwith depth vp_depth
+               [ ("O", "None")
+               ; ( "S n'"
+                 , ifthenelse depth condition
+                     (parens ~parens_req_spaces:false
+                        (econcat " "
+                           [ letin depth store_name
+                               (parens ~parens_req_spaces:false
+                                  (econcat "\n"
+                                     [body; enforce_endswith_store post] ) )
+                             (* letin depth store_name
+                                    (parens ~parens_req_spaces:false body)
+                                ; enforce_endswith_store post *)
+                           ; "loop"
+                           ; "n'" (* ; parens (id ^ " + 1") *)
+                           ; broken
+                           ; store_name ] ) )
+                     ("Some " ^ store_name) ) ] ] )
+    ; "1000%nat"
+    ; "false"
+    ; store_name ]
+
+and string_of_stmt (extract : bool) ~mid_seq bound_vars depth s =
+  (* TODO : For function calls, clear the 'result' variable after using it *)
+  let f : stmt -> string = function
+    | Nothing ->
+        (* comment "nothingn statement" *) ""
+    | Break ->
+        enforce_endswith_store (letin depth broken "true")
+    | Assignment (id, expr) -> (
+      match type_of_expr expr with
+      | Record ->
+          (* Need to find a way to unfold record fields into input variables? Idk *)
+          econcat " "
+            [ "update_record"
+            ; store_name
+            ; stringify id
+            ; string_of_expr expr false bound_vars ]
+      | _ ->
+          (* update_typctx id (type_of_expr expr) ; *)
+          let s =
+            econcat " "
+              [ "update"
+              ; store_name
+              ; stringify id
+              ; store_string_of_expr expr bound_vars ]
+          in
+          if mid_seq then letin depth store_name s else s )
+    | Sequence l ->
+        econcat "\n"
+          ( comment
+              ("Block: next " ^ string_of_int (List.length l) ^ " statements")
+          :: List.mapi
+               (fun i x ->
+                 string_of_stmt extract
+                   ~mid_seq:(i < List.length l - 1)
+                   bound_vars depth x )
+               l
+             (* @ [store_name] *) )
+    | ForLoop (id, el, eh, lb) ->
+        (* Check for bound variables *)
+        (* Currently, if X is loop iter, lifter will generate (get_int store "VP_X" which is wrong) *)
+        (* update_typctx id Z ; *)
+        let bound_vars = id :: bound_vars in
+        econcat "\n"
+          [ (* Whether the loop is iterating upwards or downwards (downto) *)
+            letin depth "going_up"
+              (string_of_expr (Lt (el, eh)) false bound_vars)
+            (* Which function to use to check if the loop bounds have been exceeded *)
+          ; letin depth "bounds_op"
+              (parens (ifthenelse ~one_line:true depth "going_up" "leb" "geb"))
+            (* Which function to use to update the loop counter *)
+          ; letin depth "iter_op"
+              (parens
+                 (ifthenelse ~one_line:true depth "going_up" "add (VInteger 1)"
+                    "sub (VInteger 1)" ) )
+            (* Set the loop variable to the low bound *)
+          ; letin depth store_name
+              (econcat " "
+                 [ "update"
+                 ; store_name
+                 ; stringify id
+                 ; store_string_of_expr el bound_vars ] )
+          ; loop
+              (* Condition *)
+              (econcat " "
+                 [ "bounds_op"
+                 ; parens
+                     ((* coq_expr_type_getter (Identifier id)
+                         ^ " " ^ *)
+                      string_of_expr (Identifier id) false
+                        bound_vars (* store_name ^ " " ^ stringify id  *) )
+                 ; parens (string_of_expr eh false bound_vars) ] )
+              ((* Loop body *)
+               string_of_stmt extract ~mid_seq:true bound_vars (depth + 1) lb )
+              (* Post-loop-body increment/decrement *)
+              (letin depth store_name
+                 (econcat " "
+                    [ "update"
+                    ; store_name
+                    ; stringify id
+                    ; parens
+                        (econcat " "
+                           [ int_expr_constr
+                           ; parens
+                               (econcat " "
+                                  [ "iter_op"
+                                  ; parens
+                                      (econcat " "
+                                         [ (* coq_expr_type_getter (Integer 0)
+                                              ; *)
+                                           store_name
+                                         ; stringify id ] ) ] ) ] ) ] ) )
+              (depth + 1) ]
+    | SideEffect e ->
+        if e = Nothing then ""
+        else
+          let content =
+            letin depth store_name (string_of_expr e false bound_vars)
+          in
+          if extract then content else comment content
+    | IfThenElse (e, st, sf) ->
+        ifthenelse depth
+          (string_of_expr e false bound_vars)
+          (string_of_stmt extract ~mid_seq bound_vars depth st)
+          ( if sf = Nothing then
+              if mid_seq then comment "nothing and mid-seq" else store_name
+            else string_of_stmt extract ~mid_seq bound_vars depth sf )
+  in
+  (* comment (string_of_stmt_type s) ^ " " ^  *)
+  f s
+
+(*
+   Return all identifiers in an expression
+*)
+and all_ids_in_expr : expr -> string list = function
+  | Integer _ | Nothing | String _ ->
+      []
+  | Identifier id ->
+      [id]
+  | Add (e1, e2)
+  | Sub (e1, e2)
+  | Gt (e1, e2)
+  | Lt (e1, e2)
+  | Eq (e1, e2)
+  | Subscript (_, e1, e2) ->
+      all_ids_in_expr e1 @ all_ids_in_expr e2
+  | ProcCall (_, e) | FuncCall (_, _, e) ->
+      List.concat (List.map all_ids_in_expr e)
+
+(*
+   Return all identifiers in a statement
+*)
+and all_ids_in_stmt : stmt -> string list = function
+  | Nothing | Break ->
+      []
+  | Assignment (_, expr) ->
+      all_ids_in_expr expr
+  | Sequence l ->
+      List.concat (List.map all_ids_in_stmt l)
+  | SideEffect expr ->
+      all_ids_in_expr expr
+  | ForLoop (_, el, eh, lb) ->
+      all_ids_in_expr el @ all_ids_in_expr eh @ all_ids_in_stmt lb
+  | IfThenElse (expr, st, sf) ->
+      all_ids_in_expr expr @ all_ids_in_stmt st @ all_ids_in_stmt sf
+
+and runtime_check = function ForLoop _ -> true | _ -> false
+
+(*
+   Wrapper for string_of_stmt that adds a "poison check," essentially capturing
+   runtime errors, including:
+
+   - Undefined variable (not a runtime error, added for practice)
+*)
+and poison_check extract bound_vars depth (stmt : stmt) =
+  (* TODO : For all stores in a statement, ensure that
+     if the ident already exists, the type of its new value
+     matches the type of its old value. If not, poisoned.
+  *)
+  if stmt = Nothing then ""
+  else
+    letins depth [store_name; poison]
+      [ ifthenelse ~noindent_first:true (depth + 1)
+          (* Add this in when more runtime checks needed *)
+          (* (econcat " "
+             ["multi_ands"; square_braces (econcat " " ["negb"; poison])] ) *)
+          (econcat " " ["negb"; poison])
+          ( if runtime_check stmt then
+              econcat " "
+                [ matchwith ~noindent_first:true depth
+                    (enforce_endswith_store
+                       (string_of_stmt extract ~mid_seq:false bound_vars
+                          (depth + 1) stmt ) )
+                    [ ("None", pair store_name "true")
+                    ; ( "Some " ^ store_name ^ "'"
+                      , pair (store_name ^ "'") poison ) ] ]
+            else
+              pair
+                ( if stmt = Nothing then store_name
+                  else
+                    enforce_endswith_store
+                      (string_of_stmt extract ~mid_seq:false bound_vars depth
+                         stmt ) )
+                poison )
+          (pair store_name "true") ]
+
+(* Generate function/procedure definitions *)
+let rec _str_of_gal_aux ?(depth = 1) (extract : bool) bound_vars = function
+  (* TODO : For functions, return should be original passed-in store with result var set,
+     should naturally handle function scopes *)
+  | Root (pt, gal) ->
+      ( false
+      , ( match pt.func_type with
+        | Procedure (id, rtl) ->
+            econcat " "
+              ( [definition_str; sanitize_id id; "(" ^ store_name ^ ": store)"]
+              @ List.mapi
+                  (fun i rt ->
+                    let t = match rt with RT n | Const n -> n | Var n -> n in
+                    econcat " "
+                      [ "("
+                      ; "arg" ^ string_of_int i
+                      ; ":"
+                      ; string_of_coq_type (coq_type_of_return_type_root t)
+                      ; ")" ] )
+                  rtl
+              @ [":="; "\n"] )
+        | Function (id, rtl, rt) ->
+            econcat " "
+              ( [definition_str; sanitize_id id; "(" ^ store_name ^ ": store)"]
+              (* Not sure how I'll handle func args yet *)
+              (* @ List.mapi
+                  (fun i rt ->
+                    let t = match rt with RT n | Const n -> n | Var n -> n in
+                    econcat " "
+                      [ "("
+                      ; "arg" ^ string_of_int i
+                      ; ":"
+                      ; string_of_coq_type (coq_type_of_return_type_root t)
+                      ; ")" ] )
+                  rtl *)
+              @ [":="; "\n"] )
+        | _ ->
+            failwith "Expected procedure or function as root node" )
+        ^ snd (_str_of_gal_aux extract bound_vars gal) )
+  | Sequence gl ->
+      ( false
+      , econcat "\n"
+          ( [letin depth poison "false"]
+          @ List.map (fun g -> snd (_str_of_gal_aux extract bound_vars g)) gl
+          @ [store_name] ) )
+  | Statement s ->
+      (false, poison_check extract bound_vars depth s)
+  | Comment s ->
+      (true, comment s)
+
+(* Entry function *)
+let string_of_gallina do_preamble fn extract extract_lang extract_path func_name
+    g gamma =
+  typctx := gamma ;
+  let is_comment, body = _str_of_gal_aux extract [] g in
+  econcat "\n"
+    [ (if do_preamble then preamble extract extract_lang else "")
+    ; (body ^ if not is_comment then "." else "")
+    ; ( if extract && not is_comment then
+          extraction fn func_name extract_lang extract_path
+        else "" ) ]
+  ^ "\n"
