theories/Volpic_preamble_list.v
@@ -1,0 +1,118 @@
+Require Import String.
+Require Import ZArith.
+Require Import List.
+Import ListNotations.
+Open Scope Z.
+Open Scope string_scope.
+Open Scope list_scope.
+
+Definition id_type := string.
+
+Inductive value : Type :=
+| VNull
+| VInteger   (n : Z)
+| VBool      (b : bool)
+| VString    (s : string)
+| VArray     (T : Type) (v : list T).
+
+Definition store : Type := (list id_type * (id_type -> value)).
+
+Definition fresh_store : store := (nil, fun _ => VNull).
+
+Definition ids : store -> list id_type := fst.
+Definition in_ids (VOLPIC_store : store) (s : id_type) :=
+    (fix f l := match l with 
+        | nil => false
+        | cons h t => if string_dec h s then true else f t
+        end) (ids VOLPIC_store).
+Definition all_in_ids (VOLPIC_store : store) (l : list id_type) :=
+    List.fold_left (
+        fun acc item => 
+            andb acc (in_ids VOLPIC_store item)
+    ) l true.
+
+Definition sf_get (VOLPIC_store : store) (s : id_type) := (snd VOLPIC_store) s.
+
+Definition get_int (VOLPIC_store : store) (s : id_type) :=
+    match sf_get VOLPIC_store s with
+    | VInteger n => n
+    | _ => 0
+    end.
+
+Definition get_string (VOLPIC_store : store) (s : id_type) :=
+    match sf_get VOLPIC_store s with
+    | VString s => s
+    | _ => EmptyString
+    end.
+
+Definition get_bool (VOLPIC_store : store) (s : id_type) :=
+    match sf_get VOLPIC_store s with
+    | VBool b => b
+    | _ => false
+    end.
+
+Definition get_array (VOLPIC_store : store) (s : id_type) :
+    list (match sf_get VOLPIC_store s with 
+     | VArray T _ => T
+     | _ => unit
+     end).
+     destruct (sf_get VOLPIC_store s);
+        try exact v;
+        exact List.nil.
+Defined.
+
+Definition subscript {T : Type} (l : list T) (idx : Z) (default : T) :=
+    let nat_idx := Z.to_nat idx in 
+    if Z.eqb (Z.of_nat nat_idx) idx then 
+        List.nth nat_idx l default
+    else
+        default.
+    (* match idx with 
+    | VInteger x => 
+        let idx := Z.to_nat x in 
+        if Z.eqb (Z.of_nat idx) x then 
+            List.nth idx l default
+        else default
+    | _ => default
+    end. *)
+
+Definition update (VOLPIC_store : store) (s : id_type) (v : value) : store :=
+    (if in_ids VOLPIC_store s then (fst VOLPIC_store) else cons s (fst VOLPIC_store), 
+    fun x => if String.eqb x s then v else (snd VOLPIC_store x)).
+
+Definition update_record (dest_store : store) (dest_prefix : id_type) (source_store : store) (source_prefix : id_type) :=
+    let record_ids := List.filter (String.prefix source_prefix) (ids source_store) in
+    List.fold_left (fun acc id => update acc (
+        String.append dest_prefix (
+            String.substring 
+                (String.length source_prefix) 
+                ((String.length id) - (String.length source_prefix)) 
+                id
+        )
+    ) (sf_get source_store id)) record_ids dest_store.
+
+Definition multi_ands bl :=
+    List.fold_left andb bl true.
+
+Require Import Coq.extraction.Extraction.
+Require Import ExtrOcamlBasic.
+Require Import ExtrOcamlString.
+Require Import ExtrOcamlZInt.
+
+Axiom string_of_char_list : string -> string.
+Extract Constant string_of_char_list => "fun cl -> (String.of_seq (List.to_seq cl))".
+
+Axiom print_endline : string -> unit.
+Extract Inlined Constant print_endline => "print_endline".
+
+Axiom print_int : Z -> unit.
+Extract Inlined Constant print_int => "print_int".
+
+Definition fpc_write_text_uint (s : store) (_ _ : Z) := s.
+Extract Inlined Constant fpc_write_text_uint => "(fun s x _ -> print_int x; s)".
+Definition fpc_writeln_end (s : store) := s.
+Extract Inlined Constant fpc_writeln_end => "(fun s -> print_endline String.empty; s)".
+
+Definition fpc_dynarray_high {T: Type} {n: nat}
+        (s : store) (l : list T) : store :=
+    update s "VP_result" (VInteger ((Z.of_nat (List.length l)) - 1)).
