theories/algos/algorithms_modified.v
@@ -1,0 +1,470 @@
+(*Preamble*)
+Require Import Volpic_preamble.
+Require Import String.
+Require Import ZArith.
+Require Import List.
+Require Import Bool.
+Require Import ExtrOcamlBasic.
+Require Import ExtrOcamlString.
+Extraction Language OCaml.
+Open Scope string_scope.
+Open Scope Z_scope.
+Import ListNotations.
+Require Import Vector.
+Import VectorNotations.
+
+Print List.nth.
+Print Vector.t.
+
+
+
+Definition print_arr {n : nat} (VP_store: store) (vec : vector Z n) := 
+	let VP_poison := false in
+	let (VP_store,VP_poison) := 
+		(if (negb VP_poison) then
+ 			 ((*Block: next 6 statements*)
+	let VP_store := fpc_write_text_char VP_store 91 0 in
+	let VP_store := fpc_write_end VP_store in VP_store,VP_poison) 
+		else
+ 			(VP_store,true)) in
+	let (VP_store,VP_poison) := 
+		(if (negb VP_poison) then
+ 			 (match 
+(let going_up := 0 <? get_int (fpc_dynarray_high VP_store vec) "VP_result" in
+		let bounds_op := (if going_up then Z.leb else Z.geb) in
+		let iter_op := (if going_up then (Z.add 1) else (Z.sub 1)) in
+		let VP_store := update VP_store "VP_I" (VInteger ( 0 )) in
+(fix loop (VP_depth : nat) (VP_broken : bool) (VP_store : store) := 
+ 			 match VP_depth with 
+ 				 | O => None
+				 | S n' => if (bounds_op (get_int VP_store "VP_I") (get_int (fpc_dynarray_high VP_store vec) "VP_result")) then
+ 				 (let VP_store := ((*Block: next 2 statements*)
+(*Block: next 6 statements*)
+			let VP_store := fpc_write_text_ansistr VP_store ((IntToStr VP_store (subscript vec (Z.to_nat (get_int VP_store "VP_I")) 0))) in
+			let VP_store := fpc_write_end VP_store in
+			let VP_store := if (get_int VP_store "VP_I" !=? get_int (fpc_dynarray_high VP_store vec) "VP_result") then
+ 	 ((*Block: next 6 statements*)
+			let VP_store := fpc_write_text_shortstr VP_store (", ") in
+			let VP_store := fpc_write_end VP_store in VP_store) 
+else
+ 	VP_store in
+		let VP_store := update VP_store "VP_I" (VInteger (iter_op (get_int VP_store "VP_I"))) in VP_store) in loop n' VP_broken VP_store) 
+			else
+ 				(Some VP_store)
+				 			 end) 1000%nat false VP_store) with 
+ 		 | None => (VP_store,true)
+		 | Some VP_store' => (VP_store',VP_poison)
+		 	 end) 
+		else
+ 			(VP_store,true)) in
+	let (VP_store,VP_poison) := 
+		(if (negb VP_poison) then
+ 			 ((*Block: next 6 statements*)
+	let VP_store := fpc_write_text_char VP_store 93 0 in
+	let VP_store := fpc_writeln_end VP_store in VP_store,VP_poison) 
+		else
+ 			(VP_store,true)) in
+VP_store.
+
+Theorem test : forall x y, (x <? y)%nat = true -> vector Z (x + (y - x))%nat -> vector Z y.
+intros. rewrite Arith_prebase.le_plus_minus_r_stt in X. exact X. 
+apply Nat.ltb_lt in H. now apply Nat.lt_le_incl in H. Defined.
+
+Require Import Lia.
+
+Definition setlength (s : store) (id : string) (new_len : nat) 
+	{old_len : nat} (old_vec : vector Z old_len) : store.
+	destruct (old_len <? new_len)%nat eqn:E.
+	- remember (append old_vec (pad_vec (new_len - old_len) 0)) as new_vec.
+	  assert (t Z new_len). {
+	 	exact (test old_len new_len E new_vec). 
+	  } exact (update s id (VArray Z new_len H)).
+	- remember (int_array_take new_len old_vec) as new_vec. 
+	  exact (update s id (VArray Z new_len new_vec)).
+Defined.
+
+Definition bubble_sort (VP_store: store) {arr_len : nat} (vec : vector Z arr_len) := 
+	let VP_poison := false in
+	(* let (VP_store, VP_poison) :=
+		if (negb VP_poison) then (
+			(setlength VP_store "VP_result" (array_size vec) (get_array VP_store "VP_result"), VP_poison)
+		) else (VP_store,true) in *)
+	let VP_store := update VP_store "VP_result" (VArray Z arr_len vec) in
+	(* Loop 1 *)
+	(* let (VP_store,VP_poison) := 
+		(if (negb VP_poison) then
+ 			 (match 
+(let going_up := 0 <? get_int (fpc_dynarray_high VP_store vec) "VP_result" in
+		let bounds_op := (if going_up then Z.leb else Z.geb) in
+		let iter_op := (if going_up then (Z.add 1) else (Z.sub 1)) in
+		let VP_store := update VP_store "VP_I" (VInteger ( 0 )) in
+(fix loop (VP_depth : nat) (VP_broken : bool) (VP_store : store) := 
+ 			 match VP_depth with 
+ 				 | O => None
+				 | S n' => if (bounds_op (get_int VP_store "VP_I") (get_int (fpc_dynarray_high VP_store vec) "VP_result")) then
+ 				 (let VP_store := (let VP_store := update VP_store (* This is a vecn id_of_parse_tree, something's gonna go wrong *)"VP_result" (VInteger ( subscript vec (Z.to_nat (get_int VP_store "VP_I")) 0 )) in
+		let VP_store := update VP_store "VP_I" (VInteger (iter_op (get_int VP_store "VP_I"))) in VP_store) in loop n' VP_broken VP_store) 
+			else
+ 				(Some VP_store)
+				 			 end) 1000%nat false VP_store) with 
+ 		 | None => (VP_store,true)
+		 | Some VP_store' => (VP_store',VP_poison)
+		 	 end)
+		else
+ 			(VP_store,true)) in *)
+	(* Outer loop *)
+	let (VP_store,VP_poison) := 
+		(if (negb VP_poison) then
+ 			 (match 
+(let going_up := get_int (fpc_dynarray_high VP_store (get_array VP_store "VP_result")) "VP_result" - 1 <? 0 in
+		let bounds_op := (if going_up then Z.leb else Z.geb) in
+		let iter_op := (if going_up then (Z.add 1) else (Z.sub 1)) in
+		let VP_store := update VP_store "VP_I" (VInteger ( get_int (fpc_dynarray_high VP_store (get_array VP_store "VP_result")) "VP_result" - 1 )) in
+		(* Inner loop*)
+		(fix loop (VP_depth : nat) (VP_broken : bool) (VP_store : store) := 
+			match VP_depth with 
+				| O => None
+				| S n' => if (bounds_op (get_int VP_store "VP_I") 0) then
+				(let VP_store := (let going_up := 0 <? get_int VP_store "VP_I" in
+			let bounds_op := (if going_up then Z.leb else Z.geb) in
+			let iter_op := (if going_up then (Z.add 1) else (Z.sub 1)) in
+			let VP_store := update VP_store "VP_J" (VInteger ( 0 )) in
+			let (VP_store,VP_poison) :=
+			match
+			((fix loop (VP_depth : nat) (VP_broken : bool) (VP_store : store) := 
+							match VP_depth with 
+								| O => None
+								| S n' => if (bounds_op (get_int VP_store "VP_J") (get_int VP_store "VP_I")) then
+								(let VP_store := (let VP_store := if (subscript (get_array VP_store "VP_result") (Z.to_nat (get_int VP_store "VP_J")) 0 >? subscript (get_array VP_store "VP_result") (Z.to_nat (get_int VP_store "VP_J" + 1)) 0) then
+				(*Block: next 3 statements*)
+							let VP_store := update VP_store "VP_TEMP" (VInteger ( subscript (get_array VP_store "VP_result") (Z.to_nat (get_int VP_store "VP_J")) 0 )) in
+							let VP_store := update VP_store "VP_result" 
+								(VArray Z arr_len (
+									(* Vector.replace_order (get_array VP_store "VP_result")) *)
+									vec
+								))
+								(* (VInteger ( subscript (get_array VP_store "VP_result") (Z.to_nat (get_int VP_store "VP_J" + 1)) 0 ))  *)
+							in
+			update VP_store "VP_result" (VInteger ( get_int VP_store "VP_TEMP" )) 
+			else
+				((*nothing and mid-seq*) VP_store) in
+						let VP_store := update VP_store "VP_J" (VInteger (iter_op (get_int VP_store "VP_J"))) in VP_store) in loop n' VP_broken VP_store) 
+							else
+								(Some VP_store)
+												end) 30%nat false VP_store) with
+			| None => (VP_store,true)
+			| Some VP_store' => (VP_store', VP_poison)
+			end in
+		(* Outer loop increment *)
+		let VP_store := update VP_store "VP_I" (VInteger (iter_op (get_int VP_store "VP_I"))) in VP_store) in loop n' VP_broken VP_store) 
+			else
+ 				(Some VP_store)
+				 			 end) 30%nat false VP_store) with 
+ 		 | None => (VP_store,true)
+		 | Some VP_store' => (VP_store',VP_poison)
+		 	 end) 
+		else
+ 			(VP_store,true)) in
+VP_store.
+Extraction "algorithms.ml" bubble_sort.
+
+(* Compute get_array (bubble_sort fresh_store [2;1]) "VP_result".
+
+Compute get_int (fpc_dynarray_high (bubble_sort fresh_store [5;3;2;1;6;8;2]) [5;3;2;1;6;8;2]) "VP_result".
+
+(* Why doesn't this return lol *)
+Compute sf_get (bubble_sort fresh_store [5;3;2;1;6;8;2]) "VP_I". *)
+
+Definition simple_loop (VP_store: store) := 
+	let VP_poison := false in
+	let (VP_store,VP_poison) := 
+		(if (negb VP_poison) then
+ 			 (match 
+(let going_up := 0 <? 10 in
+		let bounds_op := (if going_up then Z.leb else Z.geb) in
+		let iter_op := (if going_up then (Z.add 1) else (Z.sub 1)) in
+		let VP_store := update VP_store "VP_I" (VInteger ( 0 )) in
+(fix loop (VP_depth : nat) (VP_broken : bool) (VP_store : store) := 
+ 			 match VP_depth with 
+ 				 | O => None
+				 | S n' => if (bounds_op (get_int VP_store "VP_I") 10) then
+ 				 (let VP_store := ((*Block: next 6 statements*)
+			let VP_store := fpc_write_text_uint VP_store (get_int VP_store "VP_I") 0 in
+			let VP_store := fpc_writeln_end VP_store in
+		let VP_store := update VP_store "VP_I" (VInteger (iter_op (get_int VP_store "VP_I"))) in VP_store) in loop n' VP_broken VP_store) 
+			else
+ 				(Some VP_store)
+				 			 end) 1000%nat false VP_store) with 
+ 		 | None => (VP_store,true)
+		 | Some VP_store' => (VP_store',VP_poison)
+		 	 end) 
+		else
+ 			(VP_store,true)) in
+VP_store.
+Extraction "algorithms.ml" simple_loop.
+
+Definition linear_search (VP_store: store) (loop_limit : nat) {arr_len : nat} (vec : vector Z arr_len) := 
+	let VP_poison := false in
+	let (VP_store,VP_poison) := 
+		(if (negb VP_poison) then
+ 			 (update VP_store "VP_result" (VInteger ( -1 )),VP_poison) 
+		else
+ 			(VP_store,true)) in
+	let (VP_store,VP_poison) := 
+		(if (negb VP_poison) then
+ 			 (match 
+(let going_up := 0 <? Z.of_nat arr_len in
+		let bounds_op := (if going_up then Z.leb else Z.geb) in
+		let iter_op := (if going_up then (Z.add 1) else (Z.sub 1)) in
+		let VP_store := update VP_store "VP_I" (VInteger ( 0 )) in
+(fix loop (VP_depth : nat) (VP_broken : bool) (VP_store : store) := 
+ 			 match VP_depth with 
+ 				 | O => None
+				 | S n' => if (bounds_op (get_int VP_store "VP_I") (get_int (fpc_dynarray_high VP_store vec) "VP_result")) then
+ 				 (let VP_store := (let VP_store := if (subscript vec (Z.to_nat (get_int VP_store "VP_I")) 0 =? get_int VP_store "VP_KEY") then
+ 	 ((*Block: next 2 statements*)
+			let VP_store := update VP_store "VP_result" (VInteger ( get_int VP_store "VP_I" )) in
+			let VP_broken := true in VP_store) 
+else
+ 	((*nothing and mid-seq*) VP_store) in
+		let VP_store := update VP_store "VP_I" (VInteger (iter_op (get_int VP_store "VP_I"))) in VP_store) in loop n' VP_broken VP_store) 
+			else
+ 				(Some VP_store)
+				 			 end) loop_limit false VP_store) with 
+ 		 | None => (VP_store,true)
+		 | Some VP_store' => (VP_store',VP_poison)
+		 	 end) 
+		else
+ 			(VP_store,true)) in
+VP_store.
+Extraction "algorithms.ml" linear_search.
+
+Compute get_int (linear_search (update fresh_store "VP_KEY" (VInteger 3)) 10 [1;2;3;4;5]) "VP_result".
+Compute get_int (linear_search (update fresh_store "VP_KEY" (VInteger 3)) 10 []) "VP_result".
+
+Inductive list_search {A : Type} : list A -> A -> nat -> Prop :=
+  | sc_hd : forall (x : A) (xs : list A),
+      list_search (x :: xs) x 0
+  | sc_tl : forall (x y : A) (xs : list A) (n : nat),
+      list_search xs x n -> list_search (y :: xs) x (S n).
+
+Definition vector_search_correct {T : Type} {n : nat} (vec : vector T n) :=
+	list_search (Vector.to_list vec).
+
+Fixpoint vec_find {T : Type} {n : nat} (vec : vector T n) (key : T) 
+	(eq : forall n m : T, {n = m} + {n <> m}) : option nat :=
+	match vec with
+	| [] => None
+	| h :: t => if eq h key then Some O else (
+		match vec_find t key eq with
+		| None => None
+		| Some n' => Some (S n')
+		end
+	)
+	end.
+
+Theorem vec_find_correct : 
+	forall T n (vec : vector T n) key eq idx
+	(FOUND : vec_find vec key eq = Some idx),
+	vector_search_correct vec key idx.
+Proof.
+	induction vec; intros; 
+		unfold vector_search_correct in *; simpl in *.
+	- inversion FOUND.
+	- destruct (eq h key).
+		-- inversion FOUND; subst. constructor.
+		-- destruct (vec_find vec key eq) eqn:E; inversion FOUND; subst.
+			apply sc_tl, IHvec with (eq := eq), E.
+Qed.
+
+Lemma get_int_update : 
+	forall (s : store) (x : Z) (id : string),
+	get_int (update s id (VInteger x)) id = x.
+Proof.
+	intros. unfold update, get_int, sf_get.
+	simpl. rewrite String.eqb_refl. reflexivity.
+Qed.
+
+Lemma vsc_false_for_nil :
+	forall (T : Type) key idx,
+	~ (@vector_search_correct T 0 [] key idx).
+Proof.
+	intros. intro. inversion H.
+Qed.
+
+Theorem linear_search_correct_pascal :
+	forall (loop_limit : nat) (s out : store) (key : Z) (len : nat) 
+		(vec : vector Z len) (Zidx : Z)
+	(OUT : out = linear_search (update s "VP_KEY" (VInteger key)) loop_limit vec)
+	(IDX : Zidx = get_int out "VP_result")
+	(FOUND : Zidx >= 0),
+	vector_search_correct vec key (Z.to_nat Zidx).
+Proof.
+	induction loop_limit; intros; simpl in *.
+	- (* If loop limit is 0, result is always -1, which contradicts FOUND *)
+		unfold vector_search_correct, linear_search, to_list in *; simpl in *.
+		rewrite OUT in IDX. rewrite get_int_update in IDX. lia.
+	- unfold linear_search in OUT; simpl in *.
+		unfold fpc_dynarray_high in OUT. induction vec; simpl in *.
+Abort.
+	  
+
+
+
+Definition binary_search (VP_store: store) := 
+	let VP_poison := false in
+	let (VP_store,VP_poison) := 
+		(if (negb VP_poison) then
+ 			 (update VP_store "VP_L" (VInteger ( 0 )),VP_poison) 
+		else
+ 			(VP_store,true)) in
+	let (VP_store,VP_poison) := 
+		(if (negb VP_poison) then
+ 			 (update VP_store "VP_R" (VInteger ( get_int (fpc_dynarray_high VP_store (get_array VP_store "VP_ARR")) "VP_result" )),VP_poison) 
+		else
+ 			(VP_store,true)) in
+	let (VP_store,VP_poison) := 
+		(if (negb VP_poison) then
+ 			 (update VP_store "VP_result" (VInteger ( -1 )),VP_poison) 
+		else
+ 			(VP_store,true)) in
+	let (VP_store,VP_poison) := 
+		(if (negb VP_poison) then
+ 			 ((fix loop (VP_depth : nat) (VP_broken : bool) (VP_store : store) := 
+ 		 match VP_depth with 
+ 			 | O => None
+			 | S n' => if (get_int VP_store "VP_L" <=? get_int VP_store "VP_R") then
+ 			 (let VP_store := ((*Block: next 3 statements*)
+		let VP_store := update VP_store "VP_M" (VInteger ( get_int VP_store "VP_L" + get_int VP_store "VP_R" - get_int VP_store "VP_L" / 2 )) in
+		let VP_store := if (subscript (get_array VP_store "VP_ARR") (get_int VP_store "VP_M") 0 =? get_int VP_store "VP_KEY") then
+ 	 ((*Block: next 2 statements*)
+		let VP_store := update VP_store "VP_result" (VInteger ( get_int VP_store "VP_M" )) in
+		let VP_broken := true in VP_store) 
+else
+ 	((*nothing and mid-seq*) VP_store) in
+		let VP_store := if (subscript (get_array VP_store "VP_ARR") (get_int VP_store "VP_M") 0 <? get_int VP_store "VP_KEY") then
+ 	 (update VP_store "VP_L" (VInteger ( get_int VP_store "VP_M" + 1 ))) 
+else
+ 	(update VP_store "VP_R" (VInteger ( get_int VP_store "VP_M" - 1 ))) in) in loop n' VP_broken VP_store) 
+		else
+ 			(Some VP_store)
+			 		 end) 1000%nat false VP_store,VP_poison) 
+		else
+ 			(VP_store,true)) in
+VP_store.
+Extraction "algorithms.ml" binary_search.
+
+Definition main (VP_store: store) := 
+	let VP_poison := false in
+	let (VP_store,VP_poison) := 
+		(if (negb VP_poison) then
+ 			 (let VP_store := get_array (setlength VP_store 100 (get_array VP_store "VP_ARR")) "VP_result" in VP_store,VP_poison) 
+		else
+ 			(VP_store,true)) in
+	let (VP_store,VP_poison) := 
+		(if (negb VP_poison) then
+ 			 (match 
+(let going_up := 0 <? get_int (fpc_dynarray_high VP_store (get_array VP_store "VP_ARR")) "VP_result" in
+		let bounds_op := (if going_up then Z.leb else Z.geb) in
+		let iter_op := (if going_up then (Z.add 1) else (Z.sub 1)) in
+		let VP_store := update VP_store "VP_I" (VInteger ( 0 )) in
+(fix loop (VP_depth : nat) (VP_broken : bool) (VP_store : store) := 
+ 			 match VP_depth with 
+ 				 | O => None
+				 | S n' => if (bounds_op (get_int VP_store "VP_I") (get_int (fpc_dynarray_high VP_store (get_array VP_store "VP_ARR")) "VP_result")) then
+ 				 (let VP_store := (let VP_store := update VP_store "VP_(* This is a vecn id_of_parse_tree, something's gonna go wrong *)ARR" (VInteger ( get_int (Random VP_store 1000) "VP_result" )) in
+		let VP_store := update VP_store "VP_I" (VInteger (iter_op (get_int VP_store "VP_I"))) in VP_store) in loop n' VP_broken VP_store) 
+			else
+ 				(Some VP_store)
+				 			 end) 1000%nat false VP_store) with 
+ 		 | None => (VP_store,true)
+		 | Some VP_store' => (VP_store',VP_poison)
+		 	 end) 
+		else
+ 			(VP_store,true)) in
+	let (VP_store,VP_poison) := 
+		(if (negb VP_poison) then
+ 			 (update VP_store "VP_KEY" (VInteger ( subscript (get_array VP_store "VP_ARR") 50 0 )),VP_poison) 
+		else
+ 			(VP_store,true)) in
+	let (VP_store,VP_poison) := 
+		(if (negb VP_poison) then
+ 			 (update_record VP_store "VP_SORTED" (bubble_sort VP_store (get_array VP_store "VP_ARR")) "VP_result",VP_poison) 
+		else
+ 			(VP_store,true)) in
+	let (VP_store,VP_poison) := 
+		(if (negb VP_poison) then
+ 			 (update VP_store "VP_I" (VInteger ( get_int (linear_search VP_store (get_int VP_store "VP_KEY") (get_array VP_store "VP_SORTED")) "VP_result" )),VP_poison) 
+		else
+ 			(VP_store,true)) in
+	let (VP_store,VP_poison) := 
+		(if (negb VP_poison) then
+ 			 ((*Block: next 6 statements*)
+	let VP_store := fpc_write_text_shortstr VP_store ("Linear search:") 0 in
+	let VP_store := fpc_writeln_end VP_store in VP_store,VP_poison) 
+		else
+ 			(VP_store,true)) in
+	let (VP_store,VP_poison) := 
+		(if (negb VP_poison) then
+ 			 ((*Block: next 7 statements*)
+	let VP_store := fpc_write_text_shortstr VP_store ("  Key:        ") 0 in
+	let VP_store := fpc_write_text_sint VP_store (get_int VP_store "VP_KEY") 0 in
+	let VP_store := fpc_writeln_end VP_store in VP_store,VP_poison) 
+		else
+ 			(VP_store,true)) in
+	let (VP_store,VP_poison) := 
+		(if (negb VP_poison) then
+ 			 ((*Block: next 7 statements*)
+	let VP_store := fpc_write_text_shortstr VP_store ("  Index:      ") 0 in
+	let VP_store := fpc_write_text_uint VP_store (get_int VP_store "VP_I") 0 in
+	let VP_store := fpc_writeln_end VP_store in VP_store,VP_poison) 
+		else
+ 			(VP_store,true)) in
+	let (VP_store,VP_poison) := 
+		(if (negb VP_poison) then
+ 			 ((*Block: next 7 statements*)
+	let VP_store := fpc_write_text_shortstr VP_store ("  arr[index]: ") 0 in
+	let VP_store := fpc_write_text_sint VP_store (subscript (get_array VP_store "VP_SORTED") (get_int VP_store "VP_I") 0) 0 in
+	let VP_store := fpc_writeln_end VP_store in VP_store,VP_poison) 
+		else
+ 			(VP_store,true)) in
+	let (VP_store,VP_poison) := 
+		(if (negb VP_poison) then
+ 			 (update VP_store "VP_I" (VInteger ( get_int (binary_search VP_store (get_int VP_store "VP_KEY") (get_array VP_store "VP_SORTED")) "VP_result" )),VP_poison) 
+		else
+ 			(VP_store,true)) in
+	let (VP_store,VP_poison) := 
+		(if (negb VP_poison) then
+ 			 ((*Block: next 6 statements*)
+	let VP_store := fpc_write_text_shortstr VP_store ("Binary search:") 0 in
+	let VP_store := fpc_writeln_end VP_store in VP_store,VP_poison) 
+		else
+ 			(VP_store,true)) in
+	let (VP_store,VP_poison) := 
+		(if (negb VP_poison) then
+ 			 ((*Block: next 7 statements*)
+	let VP_store := fpc_write_text_shortstr VP_store ("  Key:        ") 0 in
+	let VP_store := fpc_write_text_sint VP_store (get_int VP_store "VP_KEY") 0 in
+	let VP_store := fpc_writeln_end VP_store in VP_store,VP_poison) 
+		else
+ 			(VP_store,true)) in
+	let (VP_store,VP_poison) := 
+		(if (negb VP_poison) then
+ 			 ((*Block: next 7 statements*)
+	let VP_store := fpc_write_text_shortstr VP_store ("  Index:      ") 0 in
+	let VP_store := fpc_write_text_uint VP_store (get_int VP_store "VP_I") 0 in
+	let VP_store := fpc_writeln_end VP_store in VP_store,VP_poison) 
+		else
+ 			(VP_store,true)) in
+	let (VP_store,VP_poison) := 
+		(if (negb VP_poison) then
+ 			 ((*Block: next 7 statements*)
+	let VP_store := fpc_write_text_shortstr VP_store ("  arr[index]: ") 0 in
+	let VP_store := fpc_write_text_sint VP_store (subscript (get_array VP_store "VP_SORTED") (get_int VP_store "VP_I") 0) 0 in
+	let VP_store := fpc_writeln_end VP_store in VP_store,VP_poison) 
+		else
+ 			(VP_store,true)) in
+VP_store.
+Extraction "algorithms.ml" $main.
+
+Compute (main fresh_store).
